src/QueryStructure/Implementation/Operations/General/DeleteRefinements.v
@@ -375,6 +375,51 @@ Section DeleteRefinements.
 
 End DeleteRefinements.
 
+  Ltac RemoveDeleteFunctionalDependencyCheck :=
+    match goal with
+        |- context[{b | (forall tup tup',
+                           elementIndex tup <> elementIndex tup'
+                           -> GetUnConstrRelation ?qs ?Ridx tup
+                           -> GetUnConstrRelation ?qs ?Ridx tup'
+                           -> (FunctionalDependency_P ?attrlist1 ?attrlist2 (indexedElement tup) (indexedElement tup')))
+                        -> decides b (Mutate.MutationPreservesTupleConstraints
+                                        (EnsembleDelete (GetUnConstrRelation ?qs ?Ridx) ?DeletedTuples)
+                                        (FunctionalDependency_P ?attrlist1 ?attrlist2)
+                                     )}] =>
+        let refinePK := fresh in
+        pose proof (DeletePrimaryKeysOK qs Ridx DeletedTuples attrlist1 attrlist2) as refinePK;
+          simpl in refinePK; setoid_rewrite refinePK; clear refinePK;
+          try setoid_rewrite refineEquiv_bind_unit
+    end.
+
+  Ltac ImplementDeleteForeignKeysCheck :=
+    match goal with
+        [ |- context [{b' |
+                       ?P ->
+                       decides b'
+                               (Mutate.MutationPreservesCrossConstraints
+                                  (@GetUnConstrRelation ?qs_schema ?qs ?Ridx')
+                                  (EnsembleDelete (GetUnConstrRelation ?qs ?Ridx) ?DeletedTuples)
+                                  (ForeignKey_P ?attr' ?attr ?tupmap))}]]
+        =>
+        let refineFK := fresh in
+        pose proof  (@DeleteForeignKeysCheck qs_schema qs Ridx Ridx' DeletedTuples
+                                             _ attr attr' tupmap) as refineFK;
+          simpl in refineFK; setoid_rewrite refineFK;
+          [ clear refineFK; try simplify with monad laws
+          | let tup := fresh "tup" in
+            let tup' := fresh "tup'" in
+            let tupAgree' := fresh "tupAgree'" in
+            let tupIn := fresh "tupIn" in
+            unfold tupleAgree; intros tup tup' tupAgree' tupIn;
+            rewrite tupAgree' in *;
+            [ eauto
+            | simpl; intuition]
+          | auto with typeclass_instances
+          | clear; intuition
+          | clear; simpl; intros; congruence ]
+  end.
+
 Tactic Notation "remove" "trivial" "deletion" "checks" :=
   repeat rewrite refineEquiv_bind_bind;
   etransitivity;
@@ -394,7 +439,7 @@ Tactic Notation "remove" "trivial" "deletion" "checks" :=
                    after we've drilled under a bind, this tactic will fail because
                    typeclass resolution breaks down. Generalizing and applying gets
                    around this problem for reasons unknown. *)
-        let H' := fresh in
+        let H' := fresh "H'" in
         pose proof (@QSDeleteSpec_UnConstr_refine_opt
                       _ r_n R P r_o H) as H';
           apply H'
@@ -404,7 +449,7 @@ Tactic Notation "remove" "trivial" "deletion" "checks" :=
     simpl relName in *; simpl schemaHeading in *;
     pose_string_ids; simpl;
     simplify with monad laws;
-    try rewrite <- GetRelDropConstraints;
+    repeat rewrite <- GetRelDropConstraints;
     repeat match goal with
              | H : DropQSConstraints_AbsR ?qs ?uqs |- _ =>
                rewrite H in *
@@ -414,5 +459,10 @@ Tactic Notation "remove" "trivial" "deletion" "checks" :=
 Tactic Notation "drop" "constraints" "from" "delete" constr(methname) :=
   hone method methname;
   [ remove trivial deletion checks;
+    (* Implement constraint checks. *)
+    repeat
+      first [RemoveDeleteFunctionalDependencyCheck
+            | ImplementDeleteForeignKeysCheck
+            | setoid_rewrite refine_trivial_if_then_else; simplify with monad laws];
     finish honing
   | ].
